factored out HashTree into its own module

casper/coq/theories/Casper.v
@@ -17,18 +17,13 @@ From Casper
 Require Import StrongInductionLtn.
 
 From Casper
-Require Import Quorums.
+Require Import Quorums HashTree.
 
 Set Implicit Arguments.
 Unset Strict Implicit.
 Unset Printing Implicit Defensive.
 
 Section CasperProperties.
-
-(* We consider the checkpoint tree of blocks, and so a "block" refers to a 
-   "checkpoint block" throughout the specs below. *)
-
-Variable Hash : finType.
 
 
 (* Each vote names source and target nodes by giving hash and height,
@@ -43,128 +38,6 @@ Definition Vote := (Validator * Hash * Hash * nat * nat)%type.
  *)
 
 Definition State := {fset Vote}.
-
-(* This relation links blocks (b,b') if b is an ancestor of b' and
-   b' is at the next checkpoint level above b *)
-Variable hash_parent : rel Hash.
-
-Notation "h1 <~ h2" := (hash_parent h1 h2) (at level 50).
-
-Hypothesis hash_parent_irreflexive: 
-  forall h1 h2, h1 <~ h2 -> h1 <> h2.
-
-Definition hash_ancestor h1 h2 :=
- connect hash_parent h1 h2.
-
-Notation "h1 <~* h2" := (hash_ancestor h1 h2) (at level 50).
-
-Notation "h1 </~* h2" := (~ hash_ancestor h1 h2) (at level 50).
-
-(* a hash can have one parent *)
-Hypothesis hash_at_most_one_parent :
-  forall h1 h2 h3, h2 <~ h1 -> h3 <~ h1 -> h2 = h3.
-
-(* The genesis block. *)
-Variable genesis : Hash.
-
-(* [ADDED] *)
-Hypothesis genesis_ancestor :
-  forall h, genesis <~* h.
-
-(* We will need to use several property of ancestry
-   inherited from the transitive closure operation "connect".
-   We define these lemmas rather than unfolding the hash_ancestor
-   definition inside other proofs.
- *)
-
-Lemma hash_self_ancestor :
-  forall h, h <~* h.
-Proof.
-by apply/connect0.
-Qed.
-
-Lemma hash_parent_ancestor : 
-  forall h1 h2,
-    h1 <~ h2 -> h1 <~* h2 /\ h1 <> h2.
-Proof.
-split.
-by apply/connect1.
-by apply/hash_parent_irreflexive.
-Qed.
-
-Lemma hash_ancestor_stepL : 
-  forall h1 h2 h3,
-    h1 <~ h2 -> h2 <~* h3 -> h1 <~* h3.
-Proof.
-move => h1 h2 h3.
-move/connect1.
-by apply/connect_trans.
-Qed.
-
-Lemma hash_ancestor_stepR :
-  forall h1 h2 h3, 
-    h1 <~* h2 -> h2 <~ h3 -> h1 <~* h3.
-Proof.
-move => h1 h2 h3 H1 H2.
-apply: connect_trans; eauto.
-by apply/connect1.
-Qed.
-
-Lemma hash_ancestor_concat :
-  forall h1 h2 h3, 
-    h1 <~* h2 -> h2 <~* h3 -> h1 <~* h3.
-Proof.
-move => h1 h2 h3 H2 H1.
-by apply: connect_trans; eauto.
-Qed.
-
-Lemma hash_nonancestor_nonequal:
-  forall h1 h2,
-    h1 </~* h2 -> h1 <> h2.
-Proof.
-intros h1 h2 Hna.
-contradict Hna.
-replace h1 with h2.
-apply hash_self_ancestor.
-Qed.
-
-Lemma hash_ancestor_conflict:
-  forall h1 h2 p, 
-    h1 <~* h2 -> p </~* h2 -> p </~* h1.
-Proof.
-move => h1 h2 p H1 H2 Hp.
-destruct H2.
-move: Hp H1.
-by apply/connect_trans.
-Qed.
-
-(* This definition of ancestry makes the exact number of steps explicit *)
-Inductive nth_ancestor : nat -> Hash -> Hash -> Prop :=
-| nth_ancestor_0 : forall h1, nth_ancestor 0 h1 h1
-| nth_ancestor_nth : forall n h1 h2 h3,
-    nth_ancestor n h1 h2 -> h2 <~ h3 ->
-    nth_ancestor n.+1 h1 h3.
-
-(* The nth_ancestor of t is an ancestor of t *)
-
-(* [This is roughly ancestor_means in A.S.] *)
-Lemma nth_ancestor_ancestor : 
-  forall n s t,
-    nth_ancestor n s t -> (s <~* t).
-Proof.
-  induction 1.
-  apply connect0.
-  apply connect_trans with h2;[|apply connect1];assumption.
-Qed.
-
-(* a parent is a first ancestor *)
-Example parent_ancestor : forall h1 h2,
-  h1 <~ h2 -> nth_ancestor 1 h1 h2.
-Proof.
-move => h1 h2 Hp.
-apply: nth_ancestor_nth; eauto.
-exact: nth_ancestor_0.
-Qed.
 
 (* A boolean vote_msg predicate is then a definition rather than
    a field of State as in AccountableSafety.v 
