casper/coq/theories/HashTree.v
@@ -1,0 +1,138 @@
+Set Warnings "-parsing".
+From mathcomp.ssreflect
+Require Import all_ssreflect.
+Set Warnings "parsing".
+
+From mathcomp.finmap
+Require Import finmap.
+
+Set Implicit Arguments.
+Unset Strict Implicit.
+Unset Printing Implicit Defensive.
+
+(* We consider the checkpoint tree of blocks, and so a "block" refers to a 
+   "checkpoint block" throughout the specs below. *)
+
+Parameter Hash : finType.
+
+(* This relation links blocks (b,b') if b is an ancestor of b' and
+   b' is at the next checkpoint level above b *)
+Parameter hash_parent : rel Hash.
+
+Notation "h1 <~ h2" := (hash_parent h1 h2) (at level 50).
+
+Axiom hash_parent_irreflexive: 
+  forall h1 h2, h1 <~ h2 -> h1 <> h2.
+
+Definition hash_ancestor h1 h2 :=
+ connect hash_parent h1 h2.
+
+Notation "h1 <~* h2" := (hash_ancestor h1 h2) (at level 50).
+
+Notation "h1 </~* h2" := (~ hash_ancestor h1 h2) (at level 50).
+
+(* a hash can have one parent *)
+Axiom hash_at_most_one_parent :
+  forall h1 h2 h3, h2 <~ h1 -> h3 <~ h1 -> h2 = h3.
+
+(* The genesis block. *)
+Parameter genesis : Hash.
+
+(* [ADDED] *)
+Axiom genesis_ancestor :
+  forall h, genesis <~* h.
+
+(* We will need to use several property of ancestry
+   inherited from the transitive closure operation "connect".
+   We define these lemmas rather than unfolding the hash_ancestor
+   definition inside other proofs.
+ *)
+
+Lemma hash_self_ancestor :
+  forall h, h <~* h.
+Proof.
+by apply/connect0.
+Qed.
+
+Lemma hash_parent_ancestor : 
+  forall h1 h2,
+    h1 <~ h2 -> h1 <~* h2 /\ h1 <> h2.
+Proof.
+split.
+by apply/connect1.
+by apply/hash_parent_irreflexive.
+Qed.
+
+Lemma hash_ancestor_stepL : 
+  forall h1 h2 h3,
+    h1 <~ h2 -> h2 <~* h3 -> h1 <~* h3.
+Proof.
+move => h1 h2 h3.
+move/connect1.
+by apply/connect_trans.
+Qed.
+
+Lemma hash_ancestor_stepR :
+  forall h1 h2 h3, 
+    h1 <~* h2 -> h2 <~ h3 -> h1 <~* h3.
+Proof.
+move => h1 h2 h3 H1 H2.
+apply: connect_trans; eauto.
+by apply/connect1.
+Qed.
+
+Lemma hash_ancestor_concat :
+  forall h1 h2 h3, 
+    h1 <~* h2 -> h2 <~* h3 -> h1 <~* h3.
+Proof.
+move => h1 h2 h3 H2 H1.
+by apply: connect_trans; eauto.
+Qed.
+
+Lemma hash_nonancestor_nonequal:
+  forall h1 h2,
+    h1 </~* h2 -> h1 <> h2.
+Proof.
+intros h1 h2 Hna.
+contradict Hna.
+replace h1 with h2.
+apply hash_self_ancestor.
+Qed.
+
+Lemma hash_ancestor_conflict:
+  forall h1 h2 p, 
+    h1 <~* h2 -> p </~* h2 -> p </~* h1.
+Proof.
+move => h1 h2 p H1 H2 Hp.
+destruct H2.
+move: Hp H1.
+by apply/connect_trans.
+Qed.
+
+(* This definition of ancestry makes the exact number of steps explicit *)
+Inductive nth_ancestor : nat -> Hash -> Hash -> Prop :=
+| nth_ancestor_0 : forall h1, nth_ancestor 0 h1 h1
+| nth_ancestor_nth : forall n h1 h2 h3,
+    nth_ancestor n h1 h2 -> h2 <~ h3 ->
+    nth_ancestor n.+1 h1 h3.
+
+(* The nth_ancestor of t is an ancestor of t *)
+
+(* [This is roughly ancestor_means in A.S.] *)
+Lemma nth_ancestor_ancestor : 
+  forall n s t,
+    nth_ancestor n s t -> (s <~* t).
+Proof.
+  induction 1.
+  apply connect0.
+  apply connect_trans with h2;[|apply connect1];assumption.
+Qed.
+
+(* a parent is a first ancestor *)
+Example parent_ancestor : forall h1 h2,
+  h1 <~ h2 -> nth_ancestor 1 h1 h2.
+Proof.
+move => h1 h2 Hp.
+apply: nth_ancestor_nth; eauto.
+exact: nth_ancestor_0.
+Qed.
